src/impl/TLS13.Impl.Client.fsti
@@ -92,4 +92,12 @@ fn process_local_event
           pts_to app_out app_out_bytes **
           pure (B.length network_out_bytes == SZ.v network_out_len /\
                 B.length app_out_bytes == SZ.v app_out_len /\
-                CT.some_legal_response 'st0 st1 resp network_out_bytes app_out_bytes)
+                CT.some_legal_response 'st0 st1 resp network_out_bytes app_out_bytes /\
+                CT.legal_handled_local_response
+                  'st0
+                  st1
+                  resp
+                  kind
+                  (Ghost.reveal 'payload_bytes)
+                  network_out_bytes
+                  app_out_bytes)
